src/ecSmt.ml
@@ -1445,7 +1445,7 @@ let init_relevant env pi rs =
   let push e r = r := e :: !r in
   let do1 p ax =
     let wanted = wanted_ax p in
-    if wanted || (not ax.ax_nosmt && not (unwanted_ax p)) then begin
+    if wanted || (ax.ax_visibility = `Visible && not (unwanted_ax p)) then begin
       Frequency.add fr ax;
       let used = Frequency.f_ops unwanted_ops ax.ax_spec in
       let paxu = (p,ax), used in
@@ -1576,7 +1576,7 @@ let check ?notify pi (hyps : LDecl.hyps) (concl : form) =
 
   if pi.P.pr_all then
     let init_select p ax =
-      not ax.ax_nosmt && not (P.Hints.mem p pi.P.pr_unwanted) in
+      ax.ax_visibility = `Visible && not (P.Hints.mem p pi.P.pr_unwanted) in
     (execute_task (EcEnv.Ax.all ~check:init_select env) = Some true)
   else
     let rs = Frequency.f_ops_goal unwanted_ops hyps.h_local concl in
