src/ecThCloning.mli
@@ -15,24 +15,31 @@ open EcParsetree
 type incompatible =
 | NotSameNumberOfTyParam of int * int
 | DifferentType of EcTypes.ty * EcTypes.ty
+| OpBody (* of (EcPath.path * EcDecl.operator) * (EcPath.path * EcDecl.operator) *)
+| TyBody (* of (EcPath.path * EcDecl.tydecl) * (EcPath.path * EcDecl.tydecl) *)
 
 type ovkind =
 | OVK_Type
 | OVK_Operator
 | OVK_Predicate
+| OVK_Abbrev
 | OVK_Theory
 | OVK_Lemma
+| OVK_ModExpr
+| OVK_ModType
 
 type clone_error =
-| CE_UnkTheory      of qsymbol
-| CE_DupOverride    of ovkind * qsymbol
-| CE_UnkOverride    of ovkind * qsymbol
-| CE_CrtOverride    of ovkind * qsymbol
-| CE_UnkAbbrev      of qsymbol
-| CE_TypeArgMism    of ovkind * qsymbol
-| CE_OpIncompatible of qsymbol * incompatible
-| CE_PrIncompatible of qsymbol * incompatible
-| CE_InvalidRE      of string
+| CE_UnkTheory         of qsymbol
+| CE_DupOverride       of ovkind * qsymbol
+| CE_UnkOverride       of ovkind * qsymbol
+| CE_UnkAbbrev         of qsymbol
+| CE_TypeArgMism       of ovkind * qsymbol
+| CE_OpIncompatible    of qsymbol * incompatible
+| CE_PrIncompatible    of qsymbol * incompatible
+| CE_TyIncompatible    of qsymbol * incompatible
+| CE_ModTyIncompatible of qsymbol
+| CE_ModIncompatible   of qsymbol
+| CE_InvalidRE         of string
 
 exception CloneError of EcEnv.env * clone_error
 
@@ -40,19 +47,23 @@ val clone_error : EcEnv.env -> clone_error -> 'a
 
 (* -------------------------------------------------------------------- *)
 type evclone = {
-  evc_types  : (ty_override located) Msym.t;
-  evc_ops    : (op_override located) Msym.t;
-  evc_preds  : (pr_override located) Msym.t;
-  evc_lemmas : evlemma;
-  evc_ths    : evclone Msym.t;
+  evc_types    : (ty_override located) Msym.t;
+  evc_ops      : (op_override located) Msym.t;
+  evc_preds    : (pr_override located) Msym.t;
+  evc_abbrevs  : (nt_override located) Msym.t;
+  evc_modexprs : (me_override located) Msym.t;
+  evc_modtypes : (mt_override located) Msym.t;
+  evc_lemmas   : evlemma;
+  evc_ths      : evclone Msym.t;
 }
 
 and evlemma = {
   ev_global  : (ptactic_core option * evtags option) list;
-  ev_bynames : (ptactic_core option) Msym.t;
+  ev_bynames : evinfo Msym.t;
 }
 
 and evtags = ([`Include | `Exclude] * symbol) list
+and evinfo = ptactic_core option * clmode
 
 val evc_empty : evclone
 
