src/ecTheory.ml
@@ -17,9 +17,20 @@ open EcModules
 module Sp = EcPath.Sp
 
 (* -------------------------------------------------------------------- *)
+type import = { im_immediate : bool; im_atimport : bool; }
+
+let import0  = { im_immediate =  true; im_atimport =  true; }
+let noimport = { im_immediate = false; im_atimport = false; }
+
+(* -------------------------------------------------------------------- *)
 type theory = theory_item list
 
-and theory_item =
+and theory_item = {
+  ti_item   : theory_item_r;
+  ti_import : import;
+}
+
+and theory_item_r =
   | Th_type      of (symbol * tydecl)
   | Th_operator  of (symbol * operator)
   | Th_axiom     of (symbol * axiom)
@@ -71,7 +82,12 @@ and ctheory_desc =
 
 and ctheory_struct = ctheory_item list
 
-and ctheory_item =
+and ctheory_item = {
+  cti_item   : ctheory_item_r;
+  cti_import : import;
+}
+
+and ctheory_item_r =
   | CTh_type      of (symbol * tydecl)
   | CTh_operator  of (symbol * operator)
   | CTh_axiom     of (symbol * axiom)
@@ -93,6 +109,9 @@ and ctheory_clone = {
 
 and ctheory_override =
 | CTHO_Type   of EcTypes.ty
+
+let mk_citem (import : import) (item : ctheory_item_r) =
+  { cti_import = import; cti_item = item; }
 
 (* -------------------------------------------------------------------- *)
 let module_comps_of_module_sig_comps (comps : module_sig_body) =
