src/ecUnify.mli
@@ -50,5 +50,5 @@ val tfun_expected : unienv -> EcTypes.ty list -> EcTypes.ty
 type sbody = ((EcIdent.t * ty) list * expr) Lazy.t
 
 val select_op :
-     ?filter:(operator -> bool) -> tvi -> EcEnv.env -> qsymbol -> unienv
+     ?hidden:bool -> ?filter:(operator -> bool) -> tvi -> EcEnv.env -> qsymbol -> unienv
   -> dom -> ((EcPath.path * ty list) * ty * unienv * sbody option) list
