examples/br93.ec
@@ -660,4 +660,5 @@ apply/(Reduction (A_CPA(A)) _ _ &m).
 + by move=> O O_o_ll; exact/(A_a1_ll O O_o_ll).
 by move=> O O_o_ll; proc; call (A_a2_ll O O_o_ll).
 qed.
+
 end section.
